Make mlanguage properly use angelic & demonic ND, remove unneeded definitions, introduce no-NB machinery

theories/mlanguage/mlanguage.v
@@ -18,7 +18,11 @@ Section mlanguage_mixin.
   Local Notation mixin_prog := (gmap string func).
 
   Context (apply_func : func → list val → option expr).
+  Context (expr_size : expr → nat).
   Context (head_step : mixin_prog → umrel (expr * state)).
+
+  Notation is_head_redex p x := (head_step p x (λ _, True)).
+  Notation to_val e := (match to_class e with Some (ExprVal v) => Some v | _ => None end).
 
   Record MlanguageMixin := {
     (** Expression classification *)
@@ -31,20 +35,22 @@ Section mlanguage_mixin.
       head_step p (of_class (ExprVal v), σ) X → False;
     mixin_call_head_step p f vs σ X :
       head_step p (of_class (ExprCall f vs), σ) X ↔
-      (∃ (fn : func) (e2 : expr),
-        p !! f = Some fn ∧ Some e2 = apply_func fn vs ∧ X (e2, σ));
-    mixin_call_in_ctx K K' e f vs :
-      fill K e = fill K' (of_class (ExprCall f vs)) →
-      (∃ K'', K' = comp_ectx K K'') ∨ (∃ v, of_class (ExprVal v) = e);
+      (∀ (fn : func) (e2 : expr),
+        p !! f = Some fn → Some e2 = apply_func fn vs → X (e2, σ));
 
     (** Evaluation contexts *)
     mixin_fill_empty e : fill empty_ectx e = e;
     mixin_fill_comp K1 K2 e : fill K1 (fill K2 e) = fill (comp_ectx K1 K2) e;
     mixin_fill_inj K : Inj (=) (=) (fill K);
-    (* The things in a class contain only values in redex positions (or the
+    (* The the things in a class contain only values in redex positions (or the
        redex is the topmost one). *)
     mixin_fill_class K e :
       is_Some (to_class (fill K e)) → K = empty_ectx ∨ ∃ v, to_class e = Some (ExprVal v);
+    mixin_fill_size K e :
+      K ≠ empty_ectx → expr_size e < expr_size (fill K e);
+    mixin_call_in_ctx K K' e f vs :
+      fill K e = fill K' (of_class (ExprCall f vs)) →
+      (∃ K'', K' = comp_ectx K K'') ∨ (∃ v, of_class (ExprVal v) = e);
 
     (** Given a head redex [e1_redex] somewhere in a term, and another
         decomposition of the same term into [fill K' e1'] such that [e1'] is not
@@ -54,19 +60,25 @@ Section mlanguage_mixin.
 
         This implies there can be only one head redex, see
         [head_redex_unique]. *)
-    mixin_step_by_val p K' K_redex e1' e1_redex σ X :
+    mixin_step_by_val p K' K_redex e1' e1_redex σ :
       fill K' e1' = fill K_redex e1_redex →
       match to_class e1' with Some (ExprVal _) => False | _ => True end →
-      head_step p (e1_redex, σ) X →
+      is_head_redex p (e1_redex, σ) →
       ∃ K'', K_redex = comp_ectx K' K'';
 
     (** If [fill K e] takes a head step, then either [e] is a value or [K] is
         the empty evaluation context. In other words, if [e] is not a value
         wrapping it in a context does not add new head redex positions. *)
-    (* FIXME: This is the exact same conclusion as [mixin_fill_class]... is
-       there some pattern or reduncancy here? *)
-    mixin_head_ctx_step_val p K e σ X :
-      head_step p (fill K e, σ) X → K = empty_ectx ∨ ∃ v, to_class e = Some (ExprVal v);
+    mixin_head_ctx_step_val p K e σ :
+      is_head_redex p (fill K e, σ) → K = empty_ectx ∨ ∃ v, to_class e = Some (ExprVal v);
+
+    (** If e is not head_reducible, we can recurse into it to find a head_redex in a context.
+        Since context are strictly decreasing, this implies there is no NB (except for values) *)
+    mixin_head_redex_cases p e σ : 
+      is_Some (to_val e)
+    ∨ is_head_redex p (e, σ)
+    ∨ (¬ is_head_redex p (e, σ) ∧
+        (∃ K e', e = fill K e' ∧ to_val e' = None ∧ K ≠ empty_ectx))
   }.
 End mlanguage_mixin.
 
@@ -85,24 +97,26 @@ Structure mlanguage {val : Type} := Mlanguage {
   comp_ectx : ectx → ectx → ectx;
   fill : ectx → expr → expr;
   apply_func : func → list val → option expr;
+  expr_size : expr → nat;
   head_step : mixin_prog func → umrel (expr * state);
 
   mlanguage_mixin :
     MlanguageMixin (val:=val) of_class to_class empty_ectx comp_ectx fill
-      apply_func head_step
+      apply_func expr_size head_step
 }.
 
 Declare Scope expr_scope.
 Bind Scope expr_scope with expr.
 
 Arguments mlanguage : clear implicits.
-Arguments Mlanguage {_ expr _ _ _ _ _ _ _ _ apply_func head_step}.
+Arguments Mlanguage {_ expr _ _ _ _ _ _ _ _ apply_func _ head_step}.
 Arguments of_class {_} _ _.
 Arguments to_class {_ _} _.
 Arguments empty_ectx {_ _}.
 Arguments comp_ectx {_ _} _ _.
 Arguments fill {_ _} _ _.
 Arguments apply_func {_ _}.
+Arguments expr_size {_ _} _.
 Arguments head_step {_ _} _.
 
 Definition expr_class {val} (Λ : mlanguage val) := mixin_expr_class val.
@@ -122,6 +136,8 @@ Definition to_call {val} {Λ : mlanguage val} (e : expr Λ) :=
   | _ => None
   end.
 Definition of_call {val} (Λ : mlanguage val) f (v : list val) := of_class Λ (ExprCall f v).
+
+Definition is_head_redex {val} {Λ : mlanguage val} (p : prog Λ) x := head_step p x (λ _, True).
 
 (* From an ectx_language, we can construct a mlanguage. *)
 Section mlanguage.
@@ -155,7 +171,7 @@ Section mlanguage.
   Proof. apply mlanguage_mixin. Qed.
   Lemma call_head_step p f vs σ X :
     head_step p (of_class Λ (ExprCall f vs), σ) X ↔
-    (∃ fn e2, p !! f = Some fn ∧ Some e2 = apply_func fn vs ∧ X (e2, σ)).
+    (∀ fn e2, p !! f = Some fn → Some e2 = apply_func fn vs → X (e2, σ)).
   Proof. apply mlanguage_mixin. Qed.
 
   Lemma fill_empty e : fill empty_ectx e = e.
@@ -167,14 +183,25 @@ Section mlanguage.
   Lemma fill_class' K e :
     is_Some (to_class (fill K e)) → K = empty_ectx ∨ ∃ v, to_class e = Some (ExprVal v).
   Proof. apply mlanguage_mixin. Qed.
-  Lemma step_by_val' p K' K_redex e1' e1_redex σ X :
+
+  Lemma fill_size K e :
+      K ≠ empty_ectx → expr_size e < expr_size (fill K e).
+  Proof. apply mlanguage_mixin. Qed.
+  Lemma head_redex_cases p e σ : 
+      is_Some (to_val e)
+    ∨ is_head_redex p (e, σ)
+    ∨ (¬ is_head_redex p (e, σ) ∧
+        (∃ K e', e = fill K e' ∧ to_val e' = None ∧ K ≠ empty_ectx)).
+  Proof. apply mlanguage_mixin. Qed.
+
+  Lemma step_by_val' p K' K_redex e1' e1_redex σ :
       fill K' e1' = fill K_redex e1_redex →
       match to_class e1' with Some (ExprVal _) => False | _ => True end →
-      head_step p (e1_redex, σ) X →
+      is_head_redex p (e1_redex, σ) →
       ∃ K'', K_redex = comp_ectx K' K''.
   Proof. apply mlanguage_mixin. Qed.
-  Lemma head_ctx_step_val' p K e σ X :
-    head_step p (fill K e, σ) X → K = empty_ectx ∨ ∃ v, to_class e = Some (ExprVal v).
+  Lemma head_ctx_step_val' p K e σ :
+    is_head_redex p (fill K e, σ) → K = empty_ectx ∨ ∃ v, to_class e = Some (ExprVal v).
   Proof. apply mlanguage_mixin. Qed.
   Lemma call_in_ctx K K' e f vs :
     fill K e = fill K' (of_class Λ (ExprCall f vs)) →
@@ -193,24 +220,24 @@ Section mlanguage.
     intros [?|[v Hv]]%fill_class'; first by left. right.
     rewrite /to_val Hv. eauto.
   Qed.
-  Lemma step_by_val p K' K_redex e1' e1_redex σ X :
+  Lemma step_by_val p K' K_redex e1' e1_redex σ :
       fill K' e1' = fill K_redex e1_redex →
       to_val e1' = None →
-      head_step p (e1_redex, σ) X →
+      is_head_redex p (e1_redex, σ) →
       ∃ K'', K_redex = comp_ectx K' K''.
   Proof.
     rewrite /to_val => ? He1'. eapply step_by_val'; first done.
     destruct (to_class e1') as [[]|]; done.
   Qed.
-  Lemma head_ctx_step_val p K e σ X:
-    head_step p (fill K e, σ) X → K = empty_ectx ∨ is_Some (to_val e).
+  Lemma head_ctx_step_val p K e σ:
+    is_head_redex p (fill K e, σ) → K = empty_ectx ∨ is_Some (to_val e).
   Proof.
     intros [?|[v Hv]]%head_ctx_step_val'; first by left. right.
     rewrite /to_val Hv. eauto.
   Qed.
   Lemma call_head_step_inv p f vs σ X :
     head_step p (of_class Λ (ExprCall f vs), σ) X →
-    (∃ fn e2, p !! f = Some fn ∧ Some e2 = apply_func fn vs ∧ X (e2, σ)).
+    (∀ fn e2, p !! f = Some fn → Some e2 = apply_func fn vs → X (e2, σ)).
   Proof. eapply call_head_step. Qed.
   Lemma call_head_step_intro p f vs fn σ er :
     p !! f = Some fn →
@@ -218,15 +245,13 @@ Section mlanguage.
     head_step p (of_call Λ f vs, σ) (λ '(e', σ'), e' = er ∧ σ' = σ).
   Proof.
     intros ? ?. eapply call_head_step; intros; simplify_eq.
-    do 2 eexists; repeat split; eauto.
+    split; congruence.
   Qed.
 
-  Definition head_reducible (p : prog Λ) (e : expr Λ) (σ : state Λ) :=
-    ∃ X, head_step p (e, σ) X.
-  Definition head_irreducible (p : prog Λ) (e : expr Λ) (σ : state Λ) :=
-    ∀ X, ¬head_step p (e, σ) X.
-  Definition head_stuck (p : prog Λ) (e : expr Λ) (σ : state Λ) :=
-    to_val e = None ∧ head_irreducible p e σ.
+  Lemma head_step_is_head_redex p x X : head_step p x X → is_head_redex p x.
+  Proof.
+    intros H. eapply umrel_upclosed; eauto.
+  Qed.
 
   (* All non-value redexes are at the root.  In other words, all sub-redexes are
      values. *)
@@ -247,18 +272,8 @@ Section mlanguage.
     eapply umrel_upclosed; eauto. intros [? ?]. eauto.
   Qed.
 
-  Definition reducible (p : prog Λ) (e : expr Λ) (σ : state Λ) :=
-    ∃ X, prim_step p (e, σ) X.
-  Definition irreducible (p : prog Λ) (e : expr Λ) (σ : state Λ) :=
-    ∀ X, ¬ prim_step p (e, σ) X.
-  Definition stuck (p : prog Λ) (e : expr Λ) (σ : state Λ) :=
-    to_val e = None ∧ irreducible p e σ.
-  Definition not_stuck (p : prog Λ) (e : expr Λ) (σ : state Λ) :=
-    is_Some (to_val e) ∨ reducible p e σ.
-  Definition reducible_not_ub (p : prog Λ) (e : expr Λ) (σ : state Λ) :=
-    ∃ X e' σ', prim_step p (e, σ) X ∧ X (e', σ').
-  Definition not_ub (p : prog Λ) (e : expr Λ) (σ : state Λ) :=
-    is_Some (to_val e) ∨ reducible_not_ub p e σ.
+  Definition has_ub (p : prog Λ) (e : expr Λ) (σ : state Λ) :=
+    ∃ X, prim_step p (e, σ) X ∧ ∀ x, ¬ X x.
 
   (** * Some lemmas about this language *)
   Lemma to_of_val v : to_val (of_val Λ v) = Some v.
@@ -298,58 +313,22 @@ Section mlanguage.
   Lemma of_to_call_flip f vs e : of_call Λ f vs = e → to_call e = Some (f, vs).
   Proof. intros <-. apply to_of_call. Qed.
 
-  Lemma not_reducible p e σ : ¬reducible p e σ ↔ irreducible p e σ.
-  Proof. unfold reducible, irreducible. naive_solver. Qed.
-  Lemma reducible_not_val p e σ : reducible p e σ → to_val e = None.
-  Proof. intros (?&?). eauto using val_stuck. Qed.
-  Lemma val_irreducible p e σ : is_Some (to_val e) → irreducible p e σ.
-  Proof. intros [??] ??%val_stuck. by destruct (to_val e). Qed.
   Global Instance of_val_inj : Inj (=) (=) (of_val Λ).
   Proof. by intros v v' Hv; apply (inj Some); rewrite -!to_of_val Hv. Qed.
-  Lemma not_not_stuck p e σ : ¬not_stuck p e σ ↔ stuck p e σ.
-  Proof.
-    rewrite /stuck /not_stuck -not_eq_None_Some -not_reducible.
-    destruct (decide (to_val e = None)); naive_solver.
-  Qed.
-  Lemma extcall_ctx_irreducible p K f vs σ :
+
+  Lemma extcall_ctx_has_ub p K f vs σ :
     p !! f = None →
-    irreducible p (fill K (of_class Λ (ExprCall f vs))) σ.
+    has_ub p (fill K (of_class Λ (ExprCall f vs))) σ.
   Proof.
-    intros ? X (K' & e1 & Hfill & Hstep).
-    symmetry in Hfill. pose proof (call_in_ctx_to_val _ _ _ _ _ Hfill) as [[? ->]|[? ?]].
-    - rewrite -fill_comp in Hfill. apply fill_inj in Hfill. subst e1.
-      pose proof (head_ctx_step_val _ _ _ _ _ Hstep) as [->|[? HH]].
-      + rewrite fill_empty in Hstep.
-        apply call_head_step in Hstep as (?&?&?&?&?). congruence.
-      + rewrite /to_val to_of_class // in HH.
-    - apply val_head_stuck in Hstep. congruence.
+    intros H.
+    exists (fun x => False).
+    split; last tauto.
+    econstructor. eexists; split; first done.
+    eapply call_head_step. intros ?? Hc _. rewrite H in Hc; congruence.
   Qed.
 
   Lemma fill_not_val K e : to_val e = None → to_val (fill K e) = None.
   Proof. rewrite !eq_None_not_Some. eauto using fill_val. Qed.
-
-  Lemma not_head_reducible p e σ : ¬head_reducible p e σ ↔ head_irreducible p e σ.
-  Proof. unfold head_reducible, head_irreducible. naive_solver. Qed.
-
-  (** The decomposition into head redex and context is unique.
-
-      In all sensible instances, [comp_ectx K' empty_ectx] will be the same as
-      [K'], so the conclusion is [K = K' ∧ e = e'], but we do not require a law
-      to actually prove that so we cannot use that fact here. *)
-  Lemma head_redex_unique p K K' e e' σ :
-    fill K e = fill K' e' →
-    head_reducible p e σ →
-    head_reducible p e' σ →
-    K = comp_ectx K' empty_ectx ∧ e = e'.
-  Proof.
-    intros Heq (X & Hred) (X' & Hred').
-    edestruct (step_by_val p K' K e' e) as [K'' HK];
-      [by eauto using val_head_stuck..|].
-    subst K. move: Heq. rewrite -fill_comp. intros <-%(inj (fill _)).
-    destruct (head_ctx_step_val _ _ _ _ _ Hred') as [HK''|[]%not_eq_None_Some].
-    - subst K''. rewrite fill_empty. done.
-    - by eapply val_head_stuck.
-  Qed.
 
   Lemma head_prim_step p e1 σ1 X :
     head_step p (e1, σ1) X → prim_step p (e1, σ1) X.
@@ -359,9 +338,7 @@ Section mlanguage.
     - intros *. eapply umrel_upclosed; eauto.
       intros [? ?]. rewrite fill_empty //.
   Qed.
-  Lemma head_step_not_stuck p e σ X:
-    head_step p (e, σ) X → not_stuck p e σ.
-  Proof. rewrite /not_stuck /reducible /=. eauto 10 using head_prim_step. Qed.
+
   Lemma fill_prim_step p K e1 σ1 X X' :
     (∀ e2 σ2, X (e2, σ2) → X' (fill K e2, σ2)) →
     prim_step p (e1, σ1) X →
@@ -382,21 +359,6 @@ Section mlanguage.
     - intros ? ? ?. simpl. eexists. eauto.
   Qed.
 
-  Lemma fill_reducible p K e σ : reducible p e σ → reducible p (fill K e) σ.
-  Proof.
-    intros (X & Hstep). exists (λ '(e', σ), ∃ e, e' = fill K e ∧ X (e, σ)).
-    eapply fill_prim_step; [| apply Hstep]; eauto.
-  Qed.
-  Lemma head_prim_reducible p e σ : head_reducible p e σ → reducible p e σ.
-  Proof. intros (X&?). exists X. by apply head_prim_step. Qed.
-  Lemma head_prim_fill_reducible p e K σ :
-    head_reducible p e σ → reducible p (fill K e) σ.
-  Proof. intro. by apply fill_reducible, head_prim_reducible. Qed.
-  Lemma head_prim_irreducible p e σ : irreducible p e σ → head_irreducible p e σ.
-  Proof.
-    rewrite -not_reducible -not_head_reducible. eauto using head_prim_reducible.
-  Qed.
-
   Lemma prim_head_step p e σ X :
     prim_step p (e, σ) X → sub_redexes_are_values e → head_step p (e, σ) X.
   Proof.
@@ -405,29 +367,15 @@ Section mlanguage.
     rewrite fill_empty. eapply umrel_upclosed; [apply Hstep|].
     intros [? ?]. rewrite fill_empty //.
   Qed.
-  Lemma prim_head_reducible p e σ :
-    reducible p e σ → sub_redexes_are_values e → head_reducible p e σ.
-  Proof. intros (X&Hstep) ?. eexists. by eapply prim_head_step. Qed.
-  Lemma prim_head_irreducible p e σ :
-    head_irreducible p e σ → sub_redexes_are_values e → irreducible p e σ.
-  Proof.
-    rewrite -not_reducible -not_head_reducible. eauto using prim_head_reducible.
-  Qed.
-
-  Lemma head_stuck_stuck p e σ :
-    head_stuck p e σ → sub_redexes_are_values e → stuck p e σ.
-  Proof.
-    intros [] ?. split; first done. by apply prim_head_irreducible.
-  Qed.
 
   Lemma head_reducible_prim_step_ctx p K e1 σ1 X :
-    head_reducible p e1 σ1 →
+    is_head_redex p (e1, σ1) →
     prim_step p (fill K e1, σ1) X →
     head_step p (e1, σ1) (λ '(e2', σ2), ∀ e2, e2 = fill K e2' → X (e2, σ2)).
   Proof.
-    intros (X' & HhstepK) (K' & e1' & HKe1 & Hstep).
+    intros HhstepK (K' & e1' & HKe1 & Hstep).
     edestruct (step_by_val p K) as [K'' ?];
-      eauto using val_head_stuck; simplify_eq/=.
+      eauto using val_head_stuck; simplify_eq/=; first by eapply head_step_is_head_redex.
     rewrite -fill_comp in HKe1; simplify_eq.
     apply head_ctx_step_val in HhstepK as [?|[v ?]]; simplify_eq.
     - rewrite fill_empty. eapply umrel_upclosed; [apply Hstep|].
@@ -436,7 +384,7 @@ Section mlanguage.
   Qed.
 
   Lemma head_reducible_prim_step p e1 σ1 X :
-    head_reducible p e1 σ1 →
+    is_head_redex p (e1, σ1) →
     prim_step p (e1, σ1) X →
     head_step p (e1, σ1) X.
   Proof.
@@ -445,48 +393,24 @@ Section mlanguage.
     eapply umrel_upclosed.
     - eapply Hhstep. by rewrite fill_empty.
     - intros [e σ]. rewrite fill_empty. eauto.
-  Qed.
-
-  Lemma fill_stuck (P : prog Λ) e σ K : stuck P e σ → stuck P (fill K e) σ.
-  Proof.
-    intros Hstuck; split.
-    + apply fill_not_val, Hstuck.
-    + intros X (K_redex & e1 & Heq & Hhead).
-      edestruct (step_by_val P K K_redex _ _ _ _ Heq ltac:(apply Hstuck) Hhead) as (K'' & ->).
-      rewrite -fill_comp in Heq. apply fill_inj in Heq as ->.
-      eapply (proj2 Hstuck) with (λ '(e, σ), X (fill K e, σ)).
-      do 2 eexists; split_and!; eauto.
-      eapply multirelations.umrel_upclosed; eauto. intros [? ?]. rewrite -fill_comp//.
-  Qed.
-
-  Lemma fill_not_stuck (P : prog Λ) e σ K : not_stuck P (fill K e) σ → not_stuck P e σ.
-  Proof.
-    intros [Hval | Hred].
-    - left. by eapply fill_val.
-    - destruct Hred as (X & (K_redex & e1 & Heq & Hhead)).
-      destruct (decide (to_val e = None)) as [Hnval | Hval]; first last.
-      { left. destruct (to_val e) as [v | ]; by eauto. }
-      edestruct (step_by_val P K K_redex _ _ _ _ Heq Hnval Hhead) as (K'' & ->).
-      rewrite -fill_comp in Heq. apply fill_inj in Heq as ->.
-      right. exists (λ '(e, σ), X (fill K e, σ)). do 2 eexists; split_and!; eauto.
-      eapply multirelations.umrel_upclosed; eauto. intros [? ?]. rewrite -fill_comp//.
-  Qed.
+  Qed. 
 
   Lemma prim_step_call_inv p K f vs e' σ X :
     prim_step p (fill K (of_call Λ f vs), σ) X →
-    ∃ er fn,
-      Some er = apply_func fn vs ∧ p !! f = Some fn ∧
+    ∀ er fn,
+      Some er = apply_func fn vs → p !! f = Some fn →
       X (fill K er, σ).
   Proof.
-    intros (K' & e1 & Hctx & Hstep).
-    eapply step_by_val in Hstep as H'; eauto; last apply to_val_of_call.
+    intros (K' & e1 & Hctx & Hstep) ?? Heq1 Heq2.
+    pose proof (head_step_is_head_redex _ _ _ Hstep) as Hredex.
+    eapply step_by_val in Hredex as H'; eauto; last apply to_val_of_call.
     destruct H' as [K'' Hctx']; subst K'.
     rewrite -fill_comp in Hctx. eapply fill_inj in Hctx.
     destruct (fill_class K'' e1) as [->|Hval].
     - apply is_call_is_class. erewrite of_to_call_flip; eauto.
     - rewrite fill_empty in Hctx. subst e1.
-      eapply call_head_step_inv in Hstep as (?&?&?&?&HX); simplify_eq/=.
-      rewrite -fill_comp fill_empty// in HX. eauto.
+      eapply call_head_step_inv in Hstep. 2-3:done.
+      rewrite -fill_comp fill_empty// in Hstep.
     - apply val_head_stuck in Hstep. apply not_eq_None_Some in Hval. done.
   Qed.
 
@@ -498,23 +422,7 @@ Section mlanguage.
     { rewrite -Heq. rewrite to_of_val. by exists v. }
     eapply val_head_step.
     erewrite <-(of_to_val e1') in Hstep'; eauto.
-  Qed.
-
-  Lemma fill_reducible_prim_step p e σ K X :
-    reducible p e σ →
-    prim_step p (fill K e, σ) X →
-    prim_step p (e, σ) (λ '(e2', σ2), ∀ e2, e2 = fill K e2' → X (e2, σ2)).
-  Proof.
-    intros (X'' & (K'' & e1'' & -> & Hstep)) Hprim.
-    rewrite fill_comp in Hprim.
-    eapply head_reducible_prim_step_ctx in Hprim; last by rewrite /head_reducible; eauto.
-    do 2 eexists. split_and!; eauto.
-    eapply multirelations.umrel_upclosed; [eapply Hprim|]. intros [? ?].
-    rewrite fill_comp; eauto.
-  Qed.
-
-  Lemma reducible_fill p e σ K : reducible p e σ → reducible p (fill K e) σ.
-  Proof. intros (X & Hstep). eexists. eauto using fill_prim_step'. Qed.
+  Qed. 
 
   Lemma fill_step_inv p K e1' σ1 X :
     to_val e1' = None →
@@ -522,52 +430,56 @@ Section mlanguage.
     prim_step p (e1', σ1) (λ '(e2', σ2), X (fill K e2', σ2)).
   Proof.
     intros ? (K'' & e'' & Heq & Hstep).
-    eapply step_by_val in Hstep as Hstep'; eauto. destruct Hstep' as [K' ->].
+    pose proof (head_step_is_head_redex _ _ _ Hstep) as Hredex.
+    eapply step_by_val in Hredex as Hstep'; eauto. destruct Hstep' as [K' ->].
     rewrite -fill_comp in Heq. apply (inj (fill _)) in Heq as ->.
-    do 2 eexists; split_and!; eauto.
+    do 2 eexists; split_and!; eauto. clear Hredex.
     eapply multirelations.umrel_upclosed; eauto. intros [? ?].
     rewrite -fill_comp//.
   Qed.
 
-  Lemma fill_reducible_inv p K e σ :
-    to_val e = None -> reducible p (fill K e) σ → reducible p e σ.
-  Proof. intros ? (X & Hstep%fill_step_inv); auto. eexists; eauto. Qed.
-
-  (* Lemma head_call_pure p f vs σ e2 σ' σ2 : *)
-  (*   head_step p (of_class Λ (ExprCall f vs), σ) σ e2 σ' → *)
-  (*   head_step p (of_class Λ (ExprCall f vs)) σ2 e2 σ2. *)
-  (* Proof. *)
-  (*   intros (fn & H1 & H2 & H3)%call_head_step. apply call_head_step. *)
-  (*   exists fn. repeat split; easy. *)
-  (* Qed. *)
-
   Lemma call_prim_step_fill p K f vs σ X :
     prim_step p (fill K (of_class Λ (ExprCall f vs)), σ) X →
-    ∃ (fn : func Λ) e2,
-      p !! f = Some fn ∧
-      apply_func fn vs = Some e2 ∧
+    ∀ (fn : func Λ) e2,
+      p !! f = Some fn →
+      apply_func fn vs = Some e2 →
       X (fill K e2, σ).
   Proof.
-    intros (K' & e1 & Hfill%eq_sym & Hstep).
+    intros (K' & e1 & Hfill%eq_sym & Hstep) ?? HH1 HH2.
     pose proof (call_in_ctx _ _ _ _ _ Hfill) as [[K'' ->]|[? Hval]].
     { rewrite -fill_comp in Hfill. apply fill_inj in Hfill. subst e1.
-      pose proof (head_ctx_step_val _ _ _ _ _ Hstep) as [->|[? Hval]].
-      { rewrite fill_empty in Hstep. apply call_head_step in Hstep as (fn & ? & ? & ? & ?).
-        eexists _, _; repeat split; eauto. rewrite -!fill_comp fill_empty//. }
+      pose proof (head_step_is_head_redex _ _ _ Hstep) as Hredex.
+      pose proof (head_ctx_step_val _ _ _ _ Hredex) as [->|[? Hval]].
+      { rewrite fill_empty in Hstep. eapply call_head_step in Hstep. 2-3:done.
+        rewrite -!fill_comp fill_empty//. }
       { exfalso. rewrite /to_val to_of_class// in Hval. } }
     { exfalso. subst. apply val_head_stuck in Hstep. rewrite /to_val to_of_class// in Hstep. }
   Qed.
 
   Lemma call_prim_step p f vs σ X :
     prim_step p (of_class Λ (ExprCall f vs), σ) X →
-    ∃ (fn : func Λ) e2,
-      p !! f = Some fn ∧
-      apply_func fn vs = Some e2 ∧
+    ∀ (fn : func Λ) e2,
+      p !! f = Some fn →
+      apply_func fn vs = Some e2 →
       X (e2, σ).
   Proof.
-    epose proof (call_prim_step_fill p empty_ectx _ _ _ _) as H.
-    rewrite fill_empty in H. intros (?&?&?&?&HX)%H; subst.
-    eexists _, _. repeat split; eauto. rewrite fill_empty// in HX.
+    intros H. epose proof (call_prim_step_fill p empty_ectx _ _ _ _) as Hp.
+    rewrite !fill_empty in Hp. intros fn e2 H1 H2. specialize (Hp H fn e2 H1).
+    rewrite fill_empty// in Hp. by eapply Hp.
+  Qed.
+
+  (* There is no NB *)
+  Lemma prim_step_is_total p e σ : to_val e = None → prim_step p (e,σ) (λ _, True).
+  Proof.
+    intros H.
+    induction e using (induction_ltof1 _ (expr_size)); unfold ltof in *.
+    destruct (head_redex_cases p e σ) as [(v&Hv)|[Hredex|(Hnredex&K&e'&->&He'&HK)]].
+    - congruence.
+    - eapply head_prim_step, Hredex.
+    - eapply fill_prim_step; last first; first eapply H0.
+      + by eapply fill_size.
+      + done.
+      + tauto.
   Qed.
 
   Class IntoVal (e : expr Λ) (v : val) :=
@@ -583,7 +495,7 @@ Section mlanguage.
   Qed.
 
   Record pure_step p (e1 : expr Λ) (e2 : expr Λ) := {
-    pure_step_safe σ1 : reducible p e1 σ1;
+    pure_step_not_val : to_val e1 = None;
     pure_step_det σ1 X :
       prim_step p (e1, σ1) X → X (e2, σ1)
   }.
@@ -595,10 +507,10 @@ Section mlanguage.
     PureExec φ n p e1 e2 →
     PureExec φ n p (fill K e1) (fill K e2).
   Proof.
-    intros H Hφ. specialize (H Hφ). induction H as [|n x y z [Hred Hdet] Hstep IH]; econstructor.
+    intros H Hφ. specialize (H Hφ). induction H as [|n x y z [Hval Hdet] Hstep IH]; econstructor.
     - econstructor.
-      + intros σ1. destruct (Hred σ1) as (?&H). eexists. eapply fill_prim_step'; eauto.
-      + intros σ1 X HH%fill_reducible_prim_step; last apply Hred.
+      + by eapply fill_not_val.
+      + intros σ1 X HH%fill_step_inv; last apply Hval.
         apply Hdet in HH; eauto.
     - apply IH.
   Qed.
@@ -608,9 +520,8 @@ Section mlanguage.
     pure_step p (fill K e1) (fill K e2).
   Proof.
     intros [Hred Hstep]. split.
-    - unfold reducible in *. naive_solver eauto using fill_prim_step'.
-    - intros σ1 X HstepK. specialize (Hred σ1). specialize (Hstep σ1).
-      apply fill_reducible_prim_step in HstepK; auto.
+    - by eapply fill_not_val.
+    - intros σ1 X HstepK%fill_step_inv; last done.
       apply Hstep in HstepK. eauto.
   Qed.
 
@@ -623,22 +534,6 @@ Section mlanguage.
     PureExec P n p e1 e2 →
     PureExec P n p (fill K e1) (fill K e2).
   Proof. rewrite /PureExec; eauto using pure_step_nsteps_ctx. Qed.
-
-  Record pure_head_step p (e1 : expr Λ) (e2 : expr Λ) := {
-    pure_head_step_safe σ1 : head_reducible p e1 σ1;
-    pure_head_step_det σ1 X :
-      head_step p (e1, σ1) X → X (e2, σ1)
-  }.
-
-  Lemma pure_head_step_pure_step p e1 e2 :
-    pure_head_step p e1 e2 → pure_step p e1 e2.
-  Proof.
-    intros [Hp1 Hp2]. split.
-    - intros σ. destruct (Hp1 σ) as (X & Hstep).
-      eexists. by eapply head_prim_step.
-    - intros σ X Hstep.
-      eapply head_reducible_prim_step, Hp2 in Hstep; eauto.
-  Qed.
 
 End mlanguage.
 
